small attempts at encoding choice

theories/Test.v
@@ -129,13 +129,27 @@ End Test2.
 
 Module BisimTest1.
   Inductive action : Set := | TheAction1 | TheAction2.
+
+
   Inductive term : Set :=
   | trec : term
   | tend : term
   | tfix : term -> term
   | tact : action -> term -> term
-  | tpar : action -> action -> term -> term
-  .
+  | tpar : action -> action -> term -> term.
+  (* | tcho : choice -> term
+  with choice : Type := | nil | cons (o:action -> term -> term) (t:choice).
+  (* with opt : Type := topt : action -> term -> term. *)
+
+  Example exa1 : term := tcho (cons (tact TheAction1 tend) (cons (tact TheAction2 tend) nil)).
+  Print exa1.
+
+  Notation "x :: l" := (cons x l) (at level 60, right associativity).
+  Notation "[ ]" := nil.
+  Notation "[ x ; .. ; y ]" := (cons x .. (cons y nil) ..).
+
+  Example exa2 : term := tcho [(tact TheAction1 tend); (tact TheAction2 tend)].
+  Print exa2. *)
 
   Fixpoint subst (t1 : term) (t2 : term) :=
     match t2 with
@@ -143,7 +157,11 @@ Module BisimTest1.
     | tend => tend
     | tfix t => tfix t
     | tact a t => tact a (subst t1 t)
-    | tpar a b t => tpar a b (subst t1 t)
+    (* | tpar a b t => tpar a b (subst t1 t)
+    | tcho c => match c with
+                | nil => c
+                | ()
+                end *)
     end.
 
   Inductive termLTS : term -> action -> term -> Prop :=
@@ -152,6 +170,8 @@ Module BisimTest1.
   | do_par1 : forall a b t, termLTS (tpar a b t) a (tact b t)
 
   | do_par2 : forall a b t, termLTS (tpar a b t) b (tact a t)
+
+  (* | do_cho1 : forall a b t, termLTS (tcho ) *)
 
   | do_fix : forall a t t',
       termLTS (subst (tfix t) t) a t' ->
